Switch to a global lock state
The semantics now maintains a more sensible global view of the lock in
the state: the lock is either free or some thread has it. Each thread
can project this global state into its local view (unacquired/locked),
which was the only lock state previously. This means that the lock state
can properly be used by the invariant, with "Free" having the intended
meaning of "a clean state just prior to any lock", rather than "nobody
or someone else has the lock".

Eventually this will be used to assert (at lock time) and prove (at
release time) that between write critical sections d_i = d.

src/CCLProg.v
@@ -12,18 +12,38 @@ Global Set Implicit Arguments.
 Inductive ReadState := Pending | NoReader.
 Notation DISK := (@mem addr addr_eq_dec (valu * ReadState)).
 
+Definition TID := nat.
+Opaque TID.
+
+Definition tid_eq_dec : forall (tid1 tid2:TID), {tid1=tid2}+{tid1<>tid2} :=
+  addr_eq_dec.
+
 Inductive LockState :=
-| Free
-| WriteLock.
+| Owned (tid:TID)
+| Free.
 
-Definition CanWrite (l:LockState) : {l = WriteLock} + {l <> WriteLock}.
-Proof.
-  destruct l; left + right; congruence.
-Defined.
+Inductive LocalLock :=
+| Locked
+| Unacquired.
 
-Definition lock_dec (l l':LockState) : {l=l'}+{l<>l'}.
+Definition local_l tid (l:LockState) : LocalLock :=
+  match l with
+  | Free => Unacquired
+  | Owned tid' => if tid_eq_dec tid tid' then Locked else Unacquired
+  end.
+
+Lemma local_locked : forall tid l,
+    local_l tid l = Locked ->
+    l = Owned tid.
 Proof.
-  decide equality.
+  unfold local_l; intros.
+  destruct l; simpl in *; try congruence.
+  destruct (tid_eq_dec tid tid0); subst; congruence.
+Qed.
+
+Definition lock_dec : forall (l l':LocalLock), {l=l'} + {l<>l'}.
+Proof.
+  destruct l, l'; left + right; abstract congruence.
 Defined.
 
 Polymorphic Inductive Var :=
@@ -74,9 +94,6 @@ End Sigma.
 
 Section CCL.
 
-  Definition TID := nat.
-  Opaque TID.
-
   Inductive read_transaction : Type -> Type :=
   | RDone : read_transaction unit
   | RCons : forall T, ident -> forall T', read_transaction T' -> read_transaction (T*T').
@@ -100,7 +117,7 @@ Section CCL.
   | WaitForRead (a:addr) : cprog valu
   | Write (a:addr) (v: valu) : cprog unit
   | Hash sz (buf: word sz) : cprog (word hashlen)
-  | SetLock (l:LockState) (l':LockState) : cprog unit
+  | SetLock (l:LocalLock) (l':LocalLock) : cprog unit
   | Ret T (v:T) : cprog T
   | Bind T T' (p: cprog T') (p': T' -> cprog T) : cprog T.
 
@@ -184,8 +201,8 @@ Section CCL.
       inversion H; subst; clear H; repeat Automation.inj_pair2
     end.
 
-  Ltac t' := try solve [ left; repeat deex; eauto ];
-             try (right; repeat deex; intros; inv_write_set_allocd; congruence).
+  Ltac t' := try abstract (left; repeat deex; solve [ eauto ]);
+             try abstract (right; repeat deex; intros; inv_write_set_allocd; congruence).
 
   Fixpoint wtxn_in_domain_dec (txn:write_transaction) (h:heap) {struct txn} :
     {write_set_allocd h txn} + {~write_set_allocd h txn}.
@@ -204,46 +221,46 @@ Section CCL.
         end.
   Defined.
 
-  Definition step_dec (sigma: Sigma) T (p: cprog T) : StepOutcome T :=
+  Definition step_dec tid (sigma: Sigma) T (p: cprog T) : StepOutcome T :=
     match p with
     | Alloc v => NonDet
     | ReadTxn tx => if rtxn_in_domain_dec tx (Sigma.mem sigma)
                    then NonDet (* still need to check type *)
                    else Fails
-    | AssgnTxn tx => if CanWrite (Sigma.l sigma) then
-                        if wtxn_in_domain_dec tx (Sigma.mem sigma)
-                        then NonDet (* still need to check type *)
-                        else Fails
+    | AssgnTxn tx => if local_l tid (Sigma.l sigma) then
+                      if wtxn_in_domain_dec tx (Sigma.mem sigma)
+                      then NonDet (* still need to check type *)
                       else Fails
-    | BeginRead a => if CanWrite (Sigma.l sigma) then
+                    else Fails
+    | BeginRead a => if local_l tid (Sigma.l sigma) then
                       match Sigma.disk sigma a with
                       | Some (v, NoReader) =>
                         StepTo (Sigma.upd_disk sigma (fun d => upd d a (v, Pending))) tt
                       | _ => Fails
                       end
                     else Fails
-    | WaitForRead a => if CanWrite (Sigma.l sigma) then
+    | WaitForRead a => if local_l tid (Sigma.l sigma) then
                         match Sigma.disk sigma a with
                         | Some (v, Pending) =>
                           StepTo (Sigma.upd_disk sigma (fun d => upd d a (v, NoReader))) v
                         | _ => Fails
                         end
                       else Fails
-    | Write a v => if CanWrite (Sigma.l sigma) then
+    | Write a v => if local_l tid (Sigma.l sigma) then
                     match Sigma.disk sigma a with
                     | Some (_, NoReader) =>
                       StepTo (Sigma.upd_disk sigma (fun d => upd d a (v, NoReader))) tt
                     | _ => Fails
                     end
                   else Fails
-    | SetLock l l' => if lock_dec (Sigma.l sigma) l then
+    | SetLock l l' => if lock_dec (local_l tid (Sigma.l sigma)) l then
                        match l, l' with
-                       | Free, Free => Fails
-                       | Free, WriteLock => NonDet
-                       | WriteLock, Free => NonDet (* requires guarantee proof *)
-                       | WriteLock, WriteLock => Fails
+                       | Unacquired, Unacquired => Fails
+                       | Unacquired, Locked => NonDet
+                       | Locked, Unacquired => NonDet (* requires guarantee proof *)
+                       | Locked, Locked => Fails
                        end
-                     else Fails
+                     else Fails (* caller didn't know its lock status *)
     | Ret v => StepTo sigma v
     | _ => NonDet
     end.
@@ -305,10 +322,10 @@ Section CCL.
 
   Inductive exec (tid:TID) : forall T, Sigma -> cprog T -> outcome T -> Prop :=
   | ExecStepDec : forall T (p: cprog T) sigma sigma' v,
-      step_dec sigma p = StepTo sigma' v ->
+      step_dec tid sigma p = StepTo sigma' v ->
       exec tid sigma p (Finished sigma' v)
   | ExecStepDecFail : forall T (p: cprog T) sigma,
-      step_dec sigma p = Fails ->
+      step_dec tid sigma p = Fails ->
       exec tid sigma p Error
   | ExecHash : forall sigma sz buf,
       let h := hash_fwd buf in
@@ -323,33 +340,36 @@ Section CCL.
       exec tid st p Error ->
       exec tid st (Bind p p') Error
   | ExecWriteLock : forall sigma sigma',
-      Sigma.l sigma = Free ->
+      local_l tid (Sigma.l sigma) = Unacquired ->
       Rely tid sigma sigma' ->
       hashmap_le (Sigma.hm sigma) (Sigma.hm sigma') ->
-      let sigma' := Sigma.set_l (Sigma.set_init_disk sigma' (Sigma.disk sigma')) WriteLock in
-      exec tid sigma (SetLock Free WriteLock) (Finished sigma' tt)
+      (* other threads need to release the lock before we can acquire it *)
+      Sigma.l sigma' = Free ->
+      let sigma' := Sigma.set_l (Sigma.set_init_disk sigma' (Sigma.disk sigma')) (Owned tid) in
+      exec tid sigma (SetLock Unacquired Locked) (Finished sigma' tt)
   | ExecUnlock : forall sigma out,
-      Sigma.l sigma = WriteLock ->
+      Sigma.l sigma = Owned tid ->
       let sigma' := Sigma.set_l (Sigma.set_init_disk sigma (Sigma.disk sigma)) Free in
       guarantee_exec tid sigma sigma' tt out ->
-      exec tid sigma (SetLock WriteLock Free) out
+      exec tid sigma (SetLock Locked Unacquired) out
   | ExecAlloc : forall sigma A (v:A) i,
       Sigma.mem sigma i = None ->
       let sigma' := Sigma.set_mem sigma (upd (Sigma.mem sigma) i (val v)) in
       exec tid sigma (Alloc v) (Finished sigma' i)
   | ExecReadTxn : forall sigma A (txn:read_transaction A) v sigma',
       rtxn_step txn (Sigma.mem sigma) v ->
-      (Sigma.l sigma = WriteLock -> sigma' = sigma) ->
-      (Sigma.l sigma = Free -> Rely tid sigma sigma' /\
-                      hashmap_le (Sigma.hm sigma) (Sigma.hm sigma') /\
-                      Sigma.l sigma' = Sigma.l sigma) ->
-      exec tid sigma (ReadTxn txn)
-           (Finished sigma' v)
+      (if local_l tid (Sigma.l sigma) then sigma' = sigma
+       else Rely tid sigma sigma' /\
+            (* this is essentially the lock protocol: local views of the lock do
+            not change due to other threads *)
+            local_l tid (Sigma.l sigma') = local_l tid (Sigma.l sigma) /\
+            hashmap_le (Sigma.hm sigma) (Sigma.hm sigma')) ->
+      exec tid sigma (ReadTxn txn) (Finished sigma' v)
   | ExecReadTxnFail : forall sigma A (txn:read_transaction A),
       rtxn_error txn (Sigma.mem sigma) ->
       exec tid sigma (ReadTxn txn) Error
   | ExecAssgnTxn : forall sigma (txn:write_transaction) h' out,
-      Sigma.l sigma = WriteLock ->
+      Sigma.l sigma = Owned tid ->
       wtxn_step tid txn (Sigma.mem sigma) h' ->
       let sigma' := Sigma.set_mem sigma h' in
       guarantee_exec tid sigma sigma' tt out ->
@@ -404,7 +424,7 @@ Module CCLTactics.
 
   Ltac inv_step :=
     match goal with
-    | [ H: step_dec _ _ = _ |- _ ] =>
+    | [ H: step_dec _ _ _ = _ |- _ ] =>
       simpl in H; inversion H; subst; clear H
     end.
 
@@ -421,7 +441,7 @@ Module CCLTactics.
     | [ H: exec _ _ _ (Ret _) _ |- _ ] =>
       inversion H; subst; repeat inj_pair2;
       try match goal with
-          | [ H: step_dec _ (Ret _) = _ |- _ ] =>
+          | [ H: step_dec _ _ (Ret _) = _ |- _ ] =>
             simpl in H; inversion H; subst; clear H
           end;
       clear H
@@ -439,7 +459,7 @@ Module CCLTactics.
   Ltac inv_exec' H :=
     inv_cleanup H;
     try match goal with
-        | [ H: step_dec _ _ = _ |- _ ] =>
+        | [ H: step_dec _ _ _ = _ |- _ ] =>
           simpl in H;
           repeat match goal with
                  | [ H: context[match ?d with _ => _ end] |- _ ] =>
